feat: (wip) impl `Adequacy`, pt. 3

Plfl/Untyped/BigStep.lean
@@ -15,7 +15,7 @@ open Substitution (Subst ids sub_ids)
 A closure in call-by-name is a term paired with its environment.
 -/
 inductive Clos : Type where
-| clos : ∀ {Γ}, (m : Γ ⊢ ✶) → ((Γ ∋ ✶) → Clos) → Clos
+| clos : ∀ {Γ}, (m : Γ ⊢ ✶) → (γ : (Γ ∋ ✶) → Clos) → Clos
 
 /--
 An environment in call-by-name is a mapping from variables to closures.
@@ -35,7 +35,7 @@ end Notation
 
 open Notation
 
-inductive Eval : ClosEnv Γ → (Γ ⊢ ✶) → Clos → Type where
+inductive Eval : ClosEnv Γ → (Γ ⊢ ✶) → Clos → Prop where
 | var : γ i = .clos m δ → Eval δ m v → Eval γ (` i) v
 | lam : Eval γ (ƛ m) (.clos (ƛ m) γ)
 | ap : Eval γ l (.clos (ƛ n) δ) → Eval (δ‚' .clos m γ) n v → Eval γ (l □ m) v
@@ -52,23 +52,23 @@ example
 := .ap .lam .lam
 
 -- https://plfa.github.io/BigStep/#the-big-step-semantics-is-deterministic
-theorem Eval.determ : γ ⊢ m ⇓ v → γ ⊢ m ⇓ v' → v = v' := by intro
-| .lam, .lam => rfl
-| .var h mc, .var h' mc' =>
-  injection h.symm.trans h'; rename_i h hh hh'; subst h; rw [←hh.eq, ←hh'.eq] at mc'
-  exact mc.determ mc'
-| .ap mc mc₁, .ap mc' mc₁' =>
-  have := mc.determ mc'; injection this
-  rename_i h hh hh'; subst h; rw [←hh'.eq] at mc₁'
-  injection hh; rename_i h; rw [←h] at mc₁'
-  exact mc₁.determ mc₁'
+theorem Eval.determ (e : γ ⊢ m ⇓ v) (e' : γ ⊢ m ⇓ v') : v = v' := by
+  -- generalize hx : γ = x, hx' : m = x' at *
+  induction e generalizing v' with cases e'
+  | lam => rfl
+  | var h _ ih =>
+    subst_vars; rename_i h' e'; injection h.symm.trans h'
+    rename_i h hh hh'; subst h; rw [←hh.eq, ←hh'.eq] at e'; exact ih e'
+  | ap _ _ ih ih₁ =>
+    rename_i e' e₁'; apply ih₁; injection ih e'
+    subst_vars; rename_i h; injection h; subst_vars; exact e₁'
 
 -- https://plfa.github.io/BigStep/#big-step-evaluation-implies-beta-reduction-to-a-lambda
-noncomputable def Clos.Equiv : Clos → (∅ ⊢ ✶) → Type
+noncomputable def Clos.Equiv : Clos → (∅ ⊢ ✶) → Prop
 | .clos (Γ := Γ) m γ, n =>
-  Σ (σ : Subst Γ ∅), PProd (∀ i, Clos.Equiv (γ i) (σ i)) (n = ⟪σ⟫ m)
+  ∃ (σ : Subst Γ ∅), (∀ i, Clos.Equiv (γ i) (σ i)) ∧ (n = ⟪σ⟫ m)
 
-abbrev ClosEnv.Equiv (γ : ClosEnv Γ) (σ : Subst Γ ∅) : Type :=
+abbrev ClosEnv.Equiv (γ : ClosEnv Γ) (σ : Subst Γ ∅) : Prop :=
   ∀ i, Clos.Equiv (γ i) (σ i)
 
 namespace Notation
@@ -96,18 +96,18 @@ section
   | .z => exact e
   | .s i => simp only [subst₁σ_exts]; exact ee i
 
-  theorem Eval.closEnvEquiv {γ : ClosEnv Γ} {σ : Subst Γ ∅} {m : Γ ⊢ ✶}
+  theorem Eval.clos_env_equiv {γ : ClosEnv Γ} {σ : Subst Γ ∅} {m : Γ ⊢ ✶}
   (ev : γ ⊢ m ⇓ v) (ee : γ ~~ₑ σ)
-  : Σ (n : ∅ ⊢ ✶), PProd (⟪σ⟫ m —↠ n) (v ~~ n)
-  := open Untyped.Reduce in by match ev with
-  | .lam => rename_i n; exists ⟪σ⟫ (ƛ n), by rfl, σ, ee
-  | .var h ev =>
+  : ∃ (n : ∅ ⊢ ✶), (⟪σ⟫ m —↠ n) ∧ (v ~~ n)
+  := open Untyped.Reduce in by induction ev with
+  | lam => rename_i n; exists ⟪σ⟫ (ƛ n), by rfl, σ, ee
+  | var h _ev ih =>
     rename_i i; have := ee i; rw [h] at this; have ⟨τ, eeτ, hτ⟩ := this
-    have ⟨n, rn, en⟩ := ev.closEnvEquiv eeτ; rw [←hτ] at rn; exists n, rn
-  | .ap ev ev' =>
-    have ⟨n, rn, τ, eeτ, hτ⟩ := ev.closEnvEquiv ee; subst hτ
-    have ⟨n', rn', en'⟩ := ev'.closEnvEquiv (ClosEnv.ext eeτ ⟨σ, ee, rfl⟩)
-    refine ⟨n', ?_, en'⟩; simp only [sub_ap]; rename_i n _ m
+    have ⟨n, rn, en⟩ := ih eeτ; rw [←hτ] at rn; exists n, rn
+  | ap _ev _ev' ih ih' =>
+    have ⟨n, rn, τ, eeτ, hτ⟩ := ih ee; subst hτ
+    have ⟨n', rn', en'⟩ := ih' <| ClosEnv.ext eeτ ⟨σ, ee, rfl⟩
+    refine ⟨n', ?_, en'⟩; simp only [sub_ap]; rename_i n _ m _
     apply (ap_congr₁ rn).trans; unfold ext_subst at rn'
     calc ⟪τ⟫ (ƛ n) □ ⟪σ⟫ m
       _ = (ƛ (⟪exts τ⟫ n)) □ ⟪σ⟫ m := rfl
@@ -123,7 +123,7 @@ section
   (ev : ∅ ⊢ m ⇓ .clos (ƛ n') δ)
   : ∃ (n : ∅‚ ✶ ⊢ ✶), m —↠ ƛ n
   := by
-    have ⟨n, rn, σ, _, h⟩ := ev.closEnvEquiv ClosEnv.empty_equiv_ids
+    have ⟨n, rn, σ, _, h⟩ := ev.clos_env_equiv ClosEnv.empty_equiv_ids
     subst h; rw [sub_ids] at rn; exists ⟪exts σ⟫ n'
 end
 
@@ -132,7 +132,7 @@ namespace BySubst
 
 -- https://github.com/L-TChen/ModalTypeTheory/blob/a4d3cf67236716fa324daa3e5a929f38a33c39e9/src/STLC/BigStep.agda#L96-L121
 -- https://www.cs.cornell.edu/courses/cs6110/2014sp/Handouts/Sestoft.pdf
-inductive Eval : (Γ ⊢ ✶) → (Γ ⊢ ✶) → Type where
+inductive Eval : (Γ ⊢ ✶) → (Γ ⊢ ✶) → Prop where
 -- Hmmm, it's all ƛ's after all?
 | lam : ∀ {n : ∅‚ ✶ ⊢ ✶}, Eval (ƛ n) (ƛ n)
 | ap : Eval l (ƛ m) → Eval (m⟦n⟧) v → Eval (l □ n) v
@@ -155,10 +155,11 @@ open Untyped.Subst
 If call-by-name can produce a value,
 then the program can be reduced to a λ-abstraction via β-rules.
 -/
-theorem Eval.cbn_reduce {n : ∅‚ ✶ ⊢ ✶} (ev : m ⇓' (ƛ n)) : m —↠ ƛ n := by
-  match ev with
-  | .lam => rfl
-  | .ap evl evmn' => rename_i l m n'; calc l □ n'
-      _ —↠ (ƛ m) □ n' := ap_congr₁ evl.cbn_reduce
+theorem Eval.cbn_reduce {n : Γ‚ ✶ ⊢ ✶} (ev : m ⇓' (ƛ n)) : m —↠ ƛ n := by
+  generalize hx : (ƛ n) = x, hx' : m = x' at *
+  induction ev with
+  | lam => rfl
+  | ap _evl evmn' ih ih' => subst_vars; rename_i l m n'; calc l □ n'
+      _ —↠ (ƛ m) □ n' := ap_congr₁ <| ih rfl rfl
       _ —→ m⟦n'⟧ := lamβ
-      _ —↠ (ƛ n) := evmn'.cbn_reduce
+      _ —↠ (ƛ n) := ih' rfl rfl
