Plfl/Untyped/Denotational/Adequacy.lean
@@ -8,7 +8,7 @@ namespace Adequacy
 
 open Untyped Untyped.Notation
 open Untyped.Subst
-open BigStep
+open BigStep BigStep.Notation
 open Denotational Denotational.Notation
 
 -- https://plfa.github.io/Adequacy/#the-property-of-being-greater-or-equal-to-a-function
@@ -16,7 +16,7 @@ open Denotational Denotational.Notation
 def GtFn (u : Value) : Prop := ∃ v w, v ⇾ w ⊑ u
 
 /-- If `u` is greater than a function, then an even greater value `u'` is too. -/
-theorem GtFn.sub (gt : GtFn u) (lt : u ⊑ u') : GtFn u' :=
+lemma GtFn.sub (gt : GtFn u) (lt : u ⊑ u') : GtFn u' :=
   let ⟨v, w, lt'⟩ := gt; ⟨v, w, lt'.trans lt⟩
 
 /-- `⊥` is never greater than a function. -/
@@ -25,18 +25,54 @@ lemma not_gtFn_bot : ¬ GtFn ⊥
   have ⟨_, f, s, _⟩ := sub_inv_fn lt; have ⟨_, _, i⟩ := elem_of_allFn f; cases s i
 
 /-- If the join of two values is greater than a function, then at least one of them is too. -/
-theorem GtFn.conj (gt : GtFn (u ⊔ v)) : GtFn u ∨ GtFn v := by
+lemma GtFn.conj (gt : GtFn (u ⊔ v)) : GtFn u ∨ GtFn v := by
   have ⟨_, _, lt⟩ := gt; have ⟨_, f, s, _⟩ := sub_inv_fn lt; have ⟨v, w, i⟩ := elem_of_allFn f
   refine Or.imp ?inl ?inr <| s i <;> (intro i'; exists v, w; exact sub_of_elem i')
 
 /-- If neither of the two values is greater than a function, then nor is their join. -/
 lemma not_gtFn_conj (ngt : ¬ GtFn u) (ngt' : ¬ GtFn v) : ¬ GtFn (u ⊔ v) := by
-  intro gtuv; exfalso; exact (gtuv.conj).elim ngt ngt'
+  intro gtuv; exfalso; exact gtuv.conj |>.elim ngt ngt'
 
-namespace Notation
-end Notation
+/--
+If the join of two values is not greater than a function,
+then neither of them is individually.
+-/
+lemma not_gtFn_conj_inv (ngtuv : ¬ GtFn (u ⊔ v)) : ¬ GtFn u ∧ ¬ GtFn v := by
+  by_contra h; simp_all only [not_and, not_not]
+  have ngtu := ngtuv ∘ (GtFn.sub · <| .conjR₁ .refl)
+  have ngtv := ngtuv ∘ (GtFn.sub · <| .conjR₂ .refl)
+  exact h ngtu |> ngtv
 
-open Notation
+lemma not_gtFn_conj_iff : (¬ GtFn u ∧ ¬ GtFn v) ↔ ¬ GtFn (u ⊔ v) :=
+  ⟨(λ nn => not_gtFn_conj nn.1 nn.2), not_gtFn_conj_inv⟩
 
--- open Substitution (ids sub_ids)
+theorem GtFn.dec (v : Value) : Decidable (GtFn v) := by induction v with
+| bot => left; exact not_gtFn_bot
+| fn v w => right; exists v, w
+| conj _ _ ih ih' => cases ih with
+  | isTrue h => right; have ⟨v, w, lt⟩ := h; exists v, w; exact lt.conjR₁
+  | isFalse h => cases ih' with
+    | isTrue h' => right; have ⟨v, w, lt⟩ := h'; exists v, w; exact lt.conjR₂
+    | isFalse h' => left; exact not_gtFn_conj h h'
+
+-- https://plfa.github.io/Adequacy/#relating-values-to-closures
+def 𝕍 : Value → Clos → Prop
+| _, .clos (` _) _ => ⊥
+| _, .clos (_ □ _) _ => ⊥
+| ⊥, .clos (ƛ _) _ => ⊤
+| v ⇾ w, .clos (ƛ n) γ => ∀ (c : Clos), (
+    let .clos m γ' := c
+    (GtFn v → ∃ c, (γ' ⊢ m ⇓ c) ∧ 𝕍 v c)
+    → GtFn w → ∃ c', (γ‚' c ⊢ n ⇓ c') ∧ 𝕍 w c'
+  )
+| .conj u v, c@(.clos (ƛ _) _) => 𝕍 u c ∧ 𝕍 v c
+
+def 𝔼 : Value → Clos → Prop
+| v, .clos m γ' => GtFn v → ∃ c, (γ' ⊢ m ⇓ c) ∧ 𝕍 v c
+
+-- namespace Notation
+-- end Notation
+
+-- open Notation
+
 -- open Soundness (soundness)
